add tests

tests/lean/run/iterators.lean
@@ -34,6 +34,25 @@ section ListIteratorBasic
 #guard_msgs in
 #eval [1, 2, 3].iterM IO |>.toArray
 
+example : [1, 2, 3].iter.toList = [1, 2, 3] := by
+  simp
+
+example : [1, 2, 3].iter.toArray = #[1, 2, 3] := by
+  simp
+
+example : [1, 2, 3].iter.toListRev = [3, 2, 1] := by
+  simp
+
+-- This does not work for `IO` because `LawfulMonad IO` is in Batteries
+example : ([1, 2, 3].iterM (StateM Nat)).toList = pure [1, 2, 3] := by
+  simp
+
+example : ([1, 2, 3].iterM (StateM Nat)).toArray = pure #[1, 2, 3] := by
+  simp
+
+example : ([1, 2, 3].iterM (StateM Nat)).toListRev = pure [3, 2, 1] := by
+  simp
+
 end ListIteratorBasic
 
 section WellFoundedRecursion
@@ -41,7 +60,6 @@ section WellFoundedRecursion
 def sum (l : List Nat) : Nat :=
   go l.iter 0
 where
-  @[specialize] -- The old code generator seems to need this.
   go it acc :=
     match it.step with
     | .yield it' out _ => go it' (acc + out)
@@ -63,5 +81,28 @@ def sumFold (l : List Nat) : Nat :=
 /-- info: 6 -/
 #guard_msgs in
 #eval [1, 2, 3].iter.fold (init := 0) (· + · )
+
+example (l : List Nat) : l.iter.fold (init := 0) (· + ·) = l.sum := by
+  simp [← Std.Iterators.Iter.foldl_toList, List.sum]
+  -- It remains to show that List.foldl (· + ·) = List.foldr (· + ·)
+  generalize 0 = init
+  induction l generalizing init
+  · rfl
+  · rename_i x l ih
+    simp only [List.foldl_cons, ih, List.foldr_cons]
+    clear ih
+    induction l generalizing x
+    · simp only [List.foldr_nil]
+      omega
+    · simp only [List.foldr_cons, *]
+      omega
+
+example (l : List Nat) :
+  (Id.run do
+    let mut s := 0
+    for x in l.iter do
+      s := s + x
+    return s) = l.iter.fold (init := 0) (· + ·) := by
+  simp
 
 end Loop
